| (1.43) Bernoulli's Inequality                | by-induction; multiplying by $(1+x)\geq 0$ (because $x>-1$)                                                                                                                                                                                                                                                                                                                                                                                                                                                                                                                                                                                                                                                                                                                           |
| -------------------------------------------- | ------------------------------------------------------------------------------------------------------------------------------------------------------------------------------------------------------------------------------------------------------------------------------------------------------------------------------------------------------------------------------------------------------------------------------------------------------------------------------------------------------------------------------------------------------------------------------------------------------------------------------------------------------------------------------------------------------------------------------------------------------------------------------------- |
| (1.47) Existence minimum and maximum of set  | by-induction (for max.);                                                                                                                                                                                                                                                                                                                                                                                                                                                                                                                                                                                                                                                                                                                                                              |
| (2.12) Limit Uniqueness                      | by-contra.; $\varepsilon:=\frac{\mid L_{1}-L_{2}\mid}{3}$; $n:=\max\{ N_{1},N_{2} \}+1$; trianlge ineq;                                                                                                                                                                                                                                                                                                                                                                                                                                                                                                                                                                                                                                                                               |
| (2.16) Convergent sequence is Bounded        | $\varepsilon:=1$; lim-def; triangle-ineq ($\vert{a_{n}}\vert<1+\vert{L}\vert$) ; $M:=\max\{ \vert a_{1}\vert , \dots, \vert a_{N}\vert , \vert L\vert  \}+1$; forall n: $\vert{a_{n}}\vert<M$                                                                                                                                                                                                                                                                                                                                                                                                                                                                                                                                                                                         |
| (2.22) Null * Bounded = Null                 | lim-def, $\vert{b_{n}}\vert<M$; 2.18 $\vert {a_{n}}\vert<\varepsilon\implies \vert{a_{n}}\vert<\frac{\varepsilon}{M}$                                                                                                                                                                                                                                                                                                                                                                                                                                                                                                                                                                                                                                                                 |
| (2.26)                                       | $\varepsilon:= \vert L\vert>0$ & lim-def; $\exists N:\forall n>N,\vert{b_{n}-L}\vert<\vert{L}\vert$ therefore $\vert{b_{n}}\vert\neq 0$ (2.17: foralmost=>forall);                                                                                                                                                                                                                                                                                                                                                                                                                                                                                                                                                                                                                    |
| (2.32) Squeeze Theorem                       | (2.17: foralmost=>forall); <br>$\exists(N_{1},N_{2}):\forall n>(N_{1},N_{2}),L-\varepsilon<(a_{n},c_{n})<L+\varepsilon$;<br>$N:=\max\{ N_{1},N_{2} \}\implies$<br>$\exists N\forall n>N,L-\varepsilon<a_{n}\leq b_{n}\leq c_{n}<L+\varepsilon$                                                                                                                                                                                                                                                                                                                                                                                                                                                                                                                                        |
| (2.43e) $1/\infty=0$                         | $a_{n}>K>\frac{1}{K}\implies{\frac{1}{a_{n}}<K}$                                                                                                                                                                                                                                                                                                                                                                                                                                                                                                                                                                                                                                                                                                                                      |
| 2.47                                         | we'll prove forall-n; by-induction: $0\leq\vert{a_{n}}\vert\leq\vert{a_{1}}\vert{r^{n-1}}=\frac{\vert{a_{1}}\vert}{r}{r^{n}}$; <br>$0<r<1\implies \lim{r^n}=0\underset{squeeze}{\implies} \lim{\vert a_{n}\vert }=0\underset{q{2.20}}{\implies}\lim{a_{n}}=0$                                                                                                                                                                                                                                                                                                                                                                                                                                                                                                                         |
| 3.10                                         | 3.9                                                                                                                                                                                                                                                                                                                                                                                                                                                                                                                                                                                                                                                                                                                                                                                   |
| 3.16 & 3.17                                  | 3.9                                                                                                                                                                                                                                                                                                                                                                                                                                                                                                                                                                                                                                                                                                                                                                                   |
| 3.22 (Cantor's Lemma)<br>![300](cantor.svg)  | (G1 & 3.16 $\implies$ $a_{n},b_{n}$ convergent)<br>(G2 $\implies \lim{a_{n}}=\lim{b_{n}}=:x$)<br>(3.16 $\implies$ x=sup(an)=inf(bn)$\implies a_{n}\leq x\leq b_{n}\implies{x\in{I_{n}}}$)<br>($y\in{I_{n}}\implies (a_{n}<y\leq b_{n})\underset{\text{squeeze}}{\implies}y=x\implies I_{n}=\{ x_{n} \}$)                                                                                                                                                                                                                                                                                                                                                                                                                                                                              |
| 3.32 (Bolzano–Weierstrass)<br>![120](bw.svg) | - Given $\exists a_{1},b_{1}:\forall{n},\,a_{1}\leq x_{n}\leq b_{1}$ <br>- Constract a nested-inter-seq $(I_{n}=[a_{n},b_{n}])$, which for all $n$, split $I_{n}$ into two, and set $I_{n+1}$ as the one contain infinite elements of $(x_{n})$.<br>- $\displaystyle b_{n}-a_{n}=\frac{b-a}{2^{n-1}}\underset{n \to \infty}{\longrightarrow}0\underset{\text{Cantor}}{\implies}\bigcap{\{ I_{n} \}}=\{ L=\lim_{ n \to \infty }a_{n}=\lim_{ n \to \infty }b_{n} \}$<br>- Constract $(x_{n})$-subseq $(x_{n_{k}})\to L$. (recursive: $n_{1}=1$, and define $n_{k}$ s.t. $x_{n_{k}}\in{I_{k}}$ and $n_{k}>n_{k-1}$)<br>- $a_{k}\leq x_{n_{k}}<b_{k}\underset{\text{Squeeze}}{\implies}\lim{x_{n_{k}}=L}$                                                                                 |
| 5.15 Composition Function - Continuous       | by 5.14; con-def-5.1;                                                                                                                                                                                                                                                                                                                                                                                                                                                                                                                                                                                                                                                                                                                                                                 |
| (5.29) special case of IVT for t=0           | - WLOG: $f(a)>0>f(b)$, and $[c,d]\subseteq[a,b]$ is *good* if $f(c)>0>f(d)$<br>- define intervals sequence: $I_{1}=[a,b],\,I_{n}=[a_{n},b_{n}],\,I_{n+1}=\text{good}\left\{  \left[ a_{n},m_{n} \right], \left[m_{n},b_{n} \right]\right\}$ or stop if $f(m_{n})=0$. (where $m_{n}=(a_{n}+b_{n})/2$)<br>- if $f(m_{n})=0$ for some $n$. we've found $c$.<br>- if not, $(I_{n})$ is infinite, and by Cantor $\exists c \in[a,b]:{\begin{align} c &= \lim_{ n \to \infty }a_{n} \underset{5.27}{\implies} f(c) =\lim_{ n \to \infty }f(a_{n})\geq 0 \\ c &= \lim_{ n \to \infty }b_{n} \implies f(c) =\lim_{ n \to \infty }f(b_{n})\leq 0 \end{align}}\implies{f(c)=0}$<br>- $c\in[a,b]\land f(a)>0>f(b)\implies c\in(a,b)$                                                             |
| (5.30) Existence of root for odd polynomial  | - (note: Suffice it to prove for odd degree **monic** polynomials. For general odd degree polynomials, divide by leading coefficient by the leading coefficient to get a monic polynomial which has the same roots as the original polynomial.)<br>- given $a_n=1$ and $n$ is odd.<br>$$\begin{align} P=\sum_{i=0}^{n} a_i x^i &\implies P(x)=x^n g(x)=x^n\sum_{i=0}^{n} \frac{a_{i}}{x^{n-i}}&&(x\neq 0)  \\ &\implies \lim_{x \to \infty} g(x)=\lim_{x \to -\infty} g(x)=1  \\ &\implies {(\exists M>0: \forall x, \|x\|>M \implies g(x)>0)} \\ &\implies {\begin{aligned} &\exists a<0 : P(a) = a^n g(a)<0 \\&\exists b>0 : P(b) = b^n g(b)>0\end{aligned}}&&(n \text{ is odd}) \\ &\implies P(a)P(b)<0 \\&{\implies} \exists c \in (a,b):P(c)=0 &&\text{(IVT-5.29)} \end{align}$$ |
| (5.35) W1                                    | $$\begin{align} \text{Assume } &f\text{ is unbounded on } [a,b] \\ &\implies \forall n \exists x_n \in [a,b]:\vert f(x_n)\vert>n \\ &\implies \lim_{n \to \infty} \vert f(x_n) \vert = \infty \\ &\text{Now, }  a \leq x_n \leq b  \\ &\implies   \exists x_{n_k} \to c \in [a,b] &\text{BW} \\ &\implies \lim_{k \to \infty} f(x_{n_k}) = f(c) &\text{ (5.27)} \\ &\implies \boxed {\lim_{k \to \infty} \vert f(x_{n_k}) \vert = \vert f(c) \vert}  \\ &\text{But, } \lim_{n \to \infty} \vert f(x_{n}) \vert = \infty \\ &\implies \boxed{\lim_{n \to \infty} \vert f(x_{n_k}) \vert = \infty}  &\text{Contradiction ↯}\end{align}$$                                                                                                                                                |
| (5.37) W2 (EVT)![300](w2.svg)<br>            | $$ \begin{align*} \text{Given } &f\text{ is continuous on } [a,b] \\ &\implies f\text{ is bounded on } [a,b] &\text{(W1)} \\ &\implies M:=\sup f([a,b]) \text{ exists} &\text{(3.6)} \\ &\implies \forall n \exists x_n \in [a,b]:f(x_n)>M-\frac{1}{n} &\text{(3.9)} \\ &\implies \lim_{n \to \infty} f(x_n) = M \qquad(*) &\text{(Squeeze)} \\ &\text{Also, } \exists x_{n_k} \to x_0 \in [a,b] &\text{(BW)} \\ &\implies f(x_{n_k}) \to f(x_0) &\text{(5.27)} \\ &\implies f(x_{n_k}) \to \boxed{f(x_0)=M} &\text{(3.25 and *)} \\ &\implies f \text{ attains its maximum value on } [a,b] \end{align*} $$                                                                                                                                                                          |
| (7.9) Differentiability Implies Continuity   | $$\begin{align}\displaystyle\lim_{ x \to x_{0} }(f(x)-f(x_{0}))=\lim_{ x \to x_{0} }\left( \frac{f(x)-f(x_{0})}{x-x_{0}}(x-x_{0}) \right)\implies\\\lim_{ x \to x_{0} }(f(x)-f(x_{0}))=f'(x_{0})\cdot0=0\implies\lim_{ x \to x_{0} }f(x)=f(x_{0}) \end{align}$$                                                                                                                                                                                                                                                                                                                                                                                                                                                                                                                       |
| (8.4) Fermat's Theorem                       | $$ \begin{align*} \exists N_\delta(x_0):\forall h \in (-\delta,\delta):&f(x_0+h)\leq f(x_0)\\\implies& f(x_0+h)-f(x_0)\leq0\\\implies& \begin{cases} \frac{f(x_0+h)-f(x_0)}{h}\leq0 & \text{if }h>0\\ \frac{f(x_0+h)-f(x_0)}{h}\geq0 & \text{if }h<0 \end{cases}\\\implies& f'(x_0)= \begin{cases} {f'_+(x_0)={\displaystyle\lim_{h\to0^+}}\frac{f(x_0+h)-f(x_0)}{h}\leq0} \\  {f'_-(x_0)={\displaystyle{\lim_{h\to0^-}}}\frac{f(x_0+h)-f(x_0)}{h}\geq0}\end{cases}\\\implies& \boxed{f'(x_0)=0} \end{align*} $$                                                                                                                                                                                                                                                                      |
| (8.5) Rolle's Theorem                        | $$\begin{align} m=\min f([a,b])\\ M=\max f([a,b]) &\implies &\text{(W2)}\\ \text{if }m=M&\implies\forall x \in (a,b):f(x)=M\\&\implies\exists c \in (a,b):f'(c)=0\\ \text{if }m\neq M&\implies \exists x_1,x_2 \in [a,b]:f(x_1)=m\neq f(x_2)=M \\&\implies \text{one of }x_{1},x_{2}\text{ is an inferior point} \\&\implies\exists c \in (x_1,x_2):f'(c)=0 &\text{(Fermat)} \end{align}$$                                                                                                                                                                                                                                                                                                                                                                                            |
| (8.6) Lagrange's MVT                         | $$ \begin{align} \ell(x):=\frac{f(b)-f(a)}{b-a}x+f(a) &\quad\quad\text{(Eq. of a Straight Line)} \\ g:=f(x)-\ell(x) &\implies \begin{cases} g(a)=f(a)-\ell(a)=0\\ g(b)=f(b)-\ell(b)=0 \end{cases} \\ & \implies \exists c \in (a,b) :~g'(c)=0 &\text{(Rolle)}\\ & \implies \qquad\qquad\quad f'(c)-\ell'(c)=0 \\ & \implies \qquad\qquad\quad \boxed{f'(c)=\frac{f(b)-f(a)}{b-a}} \end{align} $$                                                                                                                                                                                                                                                                                                                                                                                      |

- (4.30) (ε, δ)-definition $\iff$ Heine's definition; 
- (4.41) by contradiction: $L_{f}>L_{g}$;    $\varepsilon :=L_{f}-L_{g}$;    $\displaystyle\lim_{ x \to x_{0} }(g(x)-f(x))=L_{g}-L_{f}$;   lim-def;     ${g(x)<f(x)}$
- 4.42 h:=g-f =>L:=lim h > 0;  (lim-def(eps:=L))=>h>0=>g>f
- 8.9 Cauchy's MVT (2nd proof); 
- (8.10) Darboux's (H:=f-tx, W2 (H), Fermat (H'));   

